serialize_tags with int; proof until loop

src/Lib/DWT/ExecBer_tlv_tag_serialize.v
@@ -1,3 +1,4 @@
+Require Import VST.floyd.proofauto.
 Require Import Core.Core Core.Notations.
 
 Definition byte_length z :=
@@ -23,17 +24,54 @@ Definition ber_tlv_tag_serialize (tag size : Z): list byte * Z :=
   let tclass := tag & 3 in 
   let tval := tag >> 2 in
   if tval <=? 30 then (* Encoded in 1 octet *)
-    if negb (size =? 0) 
-    then ([Byte.repr ((tclass << 6) or tval)], 1)
-    else ([], 1)
+    if eq_dec size 0 
+    then ([], 1)
+    else ([Byte.repr ((tclass << 6) or tval)], 1) 
   else (* Encoded in > 1 octet *) 
     let required_size := byte_length tval in
-    if negb (size =? 0) 
-       then let buf0 := (tclass << 6) or 31 in
+    if eq_dec size 0 
+       then ([], required_size + 1)
+       else let buf0 := (tclass << 6) or 31 in
             if size - 1 <? required_size 
             then ([Byte.repr buf0], required_size + 1)
             else
-            (map Byte.repr (buf0 :: (serialize_tag tag)), required_size + 1)
-       else ([], required_size + 1).
+            (map Byte.repr (buf0 :: (serialize_tag tag)), required_size + 1).
 
+Open Scope IntScope.
 
+Definition byte_length' z :=
+  let fix byte_length' n z i l :=
+      match n with
+      | O => l
+      | S n => if z >> Int.repr i == 0
+               then l 
+               else byte_length' n z (i + 7)%Z (l + 1)
+      end in byte_length' 4%nat z 7 1.
+
+Definition serialize_tag' tval :=
+let fix serialize_tag' n i tval :=
+  match n with
+  | O => [tval & Int.repr 127]
+  | S n => (Int.repr 128 or (tval >> i & Int.repr 127)) 
+            :: serialize_tag' n (i - Int.repr 7) tval
+  end in 
+ let s := byte_length' tval in 
+ let n := Z.to_nat (Int.unsigned (s - 1)) in
+ serialize_tag' n (s * Int.repr  7 - Int.repr 7) tval.
+
+Definition ber_tlv_tag_serialize' (tag size : int): list int * int :=
+  let tclass := tag & Int.repr 3 in 
+  let tval := tag >> Int.repr 2 in
+  if tval <=u Int.repr 30 then
+    if eq_dec size 0 
+    then ([], 1)
+    else ([(tclass << Int.repr 6) or tval], 1) 
+  else 
+    let required_size := byte_length' tval in
+    if eq_dec size 0 
+       then ([], required_size + 1)
+       else let buf0 := (tclass << Int.repr 6) or Int.repr 31 in
+            if (size - 1 <u required_size)
+            then ([buf0], required_size + 1)
+            else
+            (buf0 :: (serialize_tag' tag), required_size + 1).
