src/Lib/DWT/VSTber_tlv_tag_serialize.v
@@ -2,9 +2,12 @@ Require Import Core.Core  Core.VstTactics Core.StructNormalizer VstLib DWT.Exec
         ErrorWithWriter.
 Require Import VST.floyd.proofauto.
 Require Import Clight.ber_tlv_tag ExecBer_tlv_tag_serialize.
+Require Import Core.Notations.
 
 Instance CompSpecs : compspecs. Proof. make_compspecs prog. Defined.
 Definition Vprog : varspecs. Proof. mk_varspecs prog. Defined.
+
+(* Open Scope Z.
 
 Definition ber_tlv_tag_serialize_spec : ident * funspec :=
   DECLARE _ber_tlv_tag_serialize
@@ -21,7 +24,11 @@ Definition ber_tlv_tag_serialize_spec : ident * funspec :=
     LOCAL(temp ret_temp (Vint (Int.repr z)))
     SEP(if eq_dec ls [] 
         then data_at_ Tsh (tarray tuchar buf_size) bufp 
-        else data_at Tsh (tarray tuint (Zlength ls)) (map Vubyte ls) bufp).
+        else data_at Tsh (tarray tuint buf_size)
+                     (map Vubyte ls ++
+                          sublist (len ls) buf_size 
+                          (default_val (tarray tuint (buf_size - len ls))))
+                     bufp).
 
 Definition Gprog := ltac:(with_library prog [ber_tlv_tag_serialize_spec]).
 
@@ -33,54 +40,137 @@ Proof.
   repeat forward.
   forward_if.
   - forward_if (
-       let (ls, z) := ber_tlv_tag_serialize tag size in
        PROP()
        LOCAL()
        SEP(if eq_dec size 0 
            then data_at_ Tsh (tarray tuchar buf_size) bufp 
-           else data_at Tsh (tarray tuint (Zlength ls)) (map Vubyte ls) bufp)).
-    + forward. break_let. 
+           else (data_at Tsh (tarray tuchar buf_size)
+    (upd_Znth 0 (default_val (tarray tuchar buf_size))
+       (Vint
+          (Int.zero_ext 8
+             (Int.or (Int.shl 
+                        (Int.repr (tag & 3)) (Int.repr 6)) 
+                     (Int.repr tag >> Int.repr 2)%int))))
+    bufp))).
+    + forward. 
       rewrite_if_b. entailer!.
-       unfold upd_Znth.
-      break_if.
-      autorewrite with sublist.
-      entailer!.
-      unfold ber_tlv_tag_serialize in *.
-      replace (Z.shiftr tag 2 <=? 30) with true in *.
-      break_if.
-      replace l with [Byte.repr (Z.lor (Z.shiftl (Z.land tag 3) 6) (Z.shiftr tag 2))].
-      entailer!.
-      unfold upd_Znth. 
-      all: admit.
-    + forward. break_let. entailer!. 
-      break_if. entailer.
-      assert (Int.unsigned (Int.repr size) = Int.unsigned (Int.repr 0)).
-      f_equal. auto.
+    + forward. entailer!. 
+      assert (Int.unsigned (Int.repr size) = Int.unsigned (Int.repr 0))
+             by (f_equal; auto).
       repeat rewrite Int.unsigned_repr_eq in *.
-      rewrite Zmod_small in *.
-      rewrite Zmod_small in *.
-      nia.
-      rep_omega.
-      nia.
+      do 2 rewrite Zmod_small in *.
+      rewrite_if_b.
+      entailer!.
+      all: rep_omega.
     + unfold POSTCONDITION.
       unfold abbreviate. 
       break_let.
       forward.
+      break_if.
+      *  unfold ber_tlv_tag_serialize in *.
+         replace (Z.shiftr tag 2 <=? 30) with true in *.
+         rewrite_if_b.
+         inversion Heqp.
+         rewrite_if_b.
+         entailer!.
+         admit.
+      * unfold ber_tlv_tag_serialize in *.
+        replace (Z.shiftr tag 2 <=? 30) with true in *.
+        rewrite_if_b.
+        inversion Heqp.
+        assert ([Byte.repr (2 * (2 * (2 * (2 * (2 * (2 * (tag & 3)))))) or (tag >> 2))] <> [])
+               by congruence.
+        rewrite_if_b.
+        entailer!. 
+        unfold upd_Znth in *.
+        break_if.
+        entailer!.
+        admit.
+        assert (buf_size = 0) as E by admit.
+        rewrite E.
+        entailer!.
+        admit.
+  - forward_if True.
+    + forward.
+      forward.
+            admit.
+    + forward. entailer!.
+    + repeat forward.
+      (* loop *)
+      admit.
+Admitted. *)
+
+Open Scope IntScope.
+
+Definition ber_tlv_tag_serialize_spec' : ident * funspec :=
+  DECLARE _ber_tlv_tag_serialize
+  WITH tag: int, bufp : val, size : int, buf_size : Z
+  PRE[tuint, tptr tvoid, tuint]
+    PROP((32 <= buf_size)%Z)
+    PARAMS(Vint tag; bufp; Vint size)
+    GLOBALS()
+    SEP(data_at_ Tsh (tarray tuchar buf_size) bufp)
+  POST[tuint]
+    let (ls, z) := ber_tlv_tag_serialize' tag size in
+    PROP()
+    LOCAL(temp ret_temp (Vint z))
+    SEP(if eq_dec ls [] 
+        then data_at_ Tsh (tarray tuchar buf_size) bufp 
+        else data_at Tsh (tarray tuchar buf_size)
+                     (map (fun x => Vint (Int.zero_ext 8 x)) ls ++
+                          sublist (len ls) buf_size 
+                          (default_val (tarray tuchar buf_size)))
+                     bufp). 
+
+Definition Gprog' := ltac:(with_library prog [ber_tlv_tag_serialize_spec']).
+
+Theorem ber_tlv_tag_serialize_correct' : 
+  semax_body Vprog Gprog' (normalize_function f_ber_tlv_tag_serialize composites)
+             ber_tlv_tag_serialize_spec'.
+Proof.
+  start_function.
+  repeat forward.
+  forward_if.
+  assert (((tag >> Int.repr 2) <=u Int.repr 30) = true) as C.
+  { unfold Int.ltu.
+    break_if;
+    autorewrite with norm in *; try nia.
+    auto.  }
+  - forward_if (
+       PROP()
+       LOCAL()
+       SEP(if eq_dec size 0 
+           then data_at_ Tsh (tarray tuchar buf_size) bufp 
+           else (data_at Tsh (tarray tuchar buf_size)
+    (upd_Znth 0 (default_val (tarray tuchar buf_size))
+       (Vint
+          (Int.zero_ext 8
+             (Int.or (Int.shl 
+                        ((tag & Int.repr 3)) (Int.repr 6)) 
+                     (tag >> Int.repr 2)%int)))) bufp))).
+    + forward. 
+      rewrite_if_b. entailer!.
+    + forward.
       rewrite_if_b.
-      break_if.
-      unfold ber_tlv_tag_serialize in *.
-      replace (Z.shiftr tag 2 <=? 30) with true in *.
-      admit.
-      admit.
-      unfold ber_tlv_tag_serialize in *.
-      replace (Z.shiftr tag 2 <=? 30) with true in *.
-      (* rewrite Heqb in *.
-      inversion Heqp.
-      break_if.
-      congruence.
-      entailer!. *)
-      admit.
-      admit.
+      entailer!.
+    + unfold POSTCONDITION.
+      unfold abbreviate. 
+      break_let.
+      forward.
+      break_if; unfold ber_tlv_tag_serialize' in *; rewrite C in *;
+        rewrite_if_b.
+      * inversion Heqp.
+        rewrite_if_b.
+        entailer!.               
+      * inversion Heqp.
+        rewrite if_false by congruence.
+        erewrite upd_Znth_unfold.
+        replace (len (default_val (tarray tuchar buf_size))) with buf_size.
+                entailer!.
+        all: unfold default_val;
+        simpl;
+        erewrite Zlength_list_repeat;
+        try nia; auto.
   - forward_if True.
     + forward.
       forward.
@@ -90,4 +180,3 @@ Proof.
       (* loop *)
       admit.
 Admitted.
-
